- A little cleanup in Classes/*. Separate standard morphisms on relf/sym/trans relations from morphisms on prop connectives and relations. - Add general order theory on predicates, instantiated for relations. Derives equivalence, implication, conjunction and disjunction as liftings from propositional connectives. Can be used for n-ary homogeneous predicates thanks to a bit of metaprogramming with lists of types. - Rebind Setoid_Theory to use the Equivalence record type instead of declaring an isomorphic one. One needs to do "red" after constructor to get the same statements when building objects of type Setoid_Theory, so scripts break.
git-svn-id: svn+ssh://scm.gforge.inria.fr/svn/coq/trunk@10765 85f007b7-540e-0410-9357-904b9bb8a0f7

toplevel/classes.ml
@@ -552,8 +552,9 @@ let new_instance ctx (instid, bk, cl) props ?(tac:Proof_type.tactic option) ?(ho
 	    let kind = Decl_kinds.Global, Decl_kinds.DefinitionBody Decl_kinds.Instance in
 	      Flags.silently (fun () ->
 		Command.start_proof id kind termtype (fun _ -> function ConstRef cst -> hook cst | _ -> assert false);
-		Pfedit.by (* (Refiner.tclTHEN (Refiner.tclEVARS (Evd.evars_of !isevars)) *)
-		  (!refine_ref (evm, term));
+		if props <> [] then 
+		  Pfedit.by (* (Refiner.tclTHEN (Refiner.tclEVARS (Evd.evars_of !isevars)) *)
+		    (!refine_ref (evm, term));
 		(match tac with Some tac -> Pfedit.by tac | None -> ())) ();
 	      Flags.if_verbose (msg $$ Printer.pr_open_subgoals) ();
 	      id
