theories/Classes/Morphisms_Prop.v
@@ -1,0 +1,131 @@
+(* -*- coq-prog-args: ("-emacs-U" "-top" "Coq.Classes.Morphisms") -*- *)
+(************************************************************************)
+(*  v      *   The Coq Proof Assistant  /  The Coq Development Team     *)
+(* <O___,, * CNRS-Ecole Polytechnique-INRIA Futurs-Universite Paris Sud *)
+(*   \VV/  **************************************************************)
+(*    //   *      This file is distributed under the terms of the       *)
+(*         *       GNU Lesser General Public License Version 2.1        *)
+(************************************************************************)
+
+(* Morphism instances for propositional connectives.
+ 
+   Author: Matthieu Sozeau
+   Institution: LRI, CNRS UMR 8623 - UniversitÃcopyright Paris Sud
+   91405 Orsay, France *)
+
+Require Import Coq.Classes.Morphisms.
+Require Import Coq.Program.Program.
+
+(** Standard instances for [not], [iff] and [impl]. *)
+
+(** Logical negation. *)
+
+Program Instance not_impl_morphism :
+  Morphism (impl --> impl) not.
+
+Program Instance not_iff_morphism : 
+  Morphism (iff ++> iff) not.
+
+(** Logical conjunction. *)
+
+Program Instance and_impl_iff_morphism :
+  Morphism (impl ==> impl ==> impl) and.
+
+(* Program Instance and_impl_iff_morphism :  *)
+(*   Morphism (impl ==> iff ==> impl) and. *)
+
+(* Program Instance and_iff_impl_morphism :  *)
+(*   Morphism (iff ==> impl ==> impl) and. *)
+
+(* Program Instance and_inverse_impl_iff_morphism :  *)
+(*   Morphism (inverse impl ==> iff ==> inverse impl) and. *)
+
+(* Program Instance and_iff_inverse_impl_morphism :  *)
+(*   Morphism (iff ==> inverse impl ==> inverse impl) and. *)
+
+Program Instance and_iff_morphism : 
+  Morphism (iff ==> iff ==> iff) and.
+
+(** Logical disjunction. *)
+
+Program Instance or_impl_iff_morphism : 
+  Morphism (impl ==> impl ==> impl) or.
+
+(* Program Instance or_impl_iff_morphism :  *)
+(*   Morphism (impl ==> iff ==> impl) or. *)
+
+(* Program Instance or_iff_impl_morphism :  *)
+(*   Morphism (iff ==> impl ==> impl) or. *)
+
+(* Program Instance or_inverse_impl_iff_morphism : *)
+(*   Morphism (inverse impl ==> iff ==> inverse impl) or. *)
+
+(* Program Instance or_iff_inverse_impl_morphism :  *)
+(*   Morphism (iff ==> inverse impl ==> inverse impl) or. *)
+
+Program Instance or_iff_morphism : 
+  Morphism (iff ==> iff ==> iff) or.
+
+(** Logical implication [impl] is a morphism for logical equivalence. *)
+
+Program Instance iff_iff_iff_impl_morphism : Morphism (iff ==> iff ==> iff) impl.
+
+(** Morphisms for quantifiers *)
+
+Program Instance {A : Type} => ex_iff_morphism : Morphism (pointwise_relation iff ==> iff) (@ex A).
+
+  Next Obligation.
+  Proof.
+    unfold pointwise_relation in H.     
+    split ; intros.
+    destruct H0 as [x₁ H₁].
+    exists x₁. rewrite H in H₁. assumption.
+    
+    destruct H0 as [x₁ H₁].
+    exists x₁. rewrite H. assumption.
+  Qed.
+
+Program Instance {A : Type} => ex_impl_morphism :
+  Morphism (pointwise_relation impl ==> impl) (@ex A).
+
+  Next Obligation.
+  Proof.
+    unfold pointwise_relation in H.  
+    exists H0. apply H. assumption.
+  Qed.
+
+Program Instance {A : Type} => ex_inverse_impl_morphism : 
+  Morphism (pointwise_relation (inverse impl) ==> inverse impl) (@ex A).
+
+  Next Obligation.
+  Proof.
+    unfold pointwise_relation in H.  
+    exists H0. apply H. assumption.
+  Qed.
+
+Program Instance {A : Type} => all_iff_morphism : 
+  Morphism (pointwise_relation iff ==> iff) (@all A).
+
+  Next Obligation.
+  Proof.
+    unfold pointwise_relation, all in *.
+    intuition ; specialize (H x0) ; intuition.
+  Qed.
+
+Program Instance {A : Type} => all_impl_morphism : 
+  Morphism (pointwise_relation impl ==> impl) (@all A).
+  
+  Next Obligation.
+  Proof.
+    unfold pointwise_relation, all in *.
+    intuition ; specialize (H x0) ; intuition.
+  Qed.
+
+Program Instance {A : Type} => all_inverse_impl_morphism : 
+  Morphism (pointwise_relation (inverse impl) ==> inverse impl) (@all A).
+  
+  Next Obligation.
+  Proof.
+    unfold pointwise_relation, all in *.
+    intuition ; specialize (H x0) ; intuition.
+  Qed.
