theories/Classes/Morphisms_Relations.v
@@ -1,0 +1,47 @@
+(* -*- coq-prog-args: ("-emacs-U" "-top" "Coq.Classes.Morphisms") -*- *)
+(************************************************************************)
+(*  v      *   The Coq Proof Assistant  /  The Coq Development Team     *)
+(* <O___,, * CNRS-Ecole Polytechnique-INRIA Futurs-Universite Paris Sud *)
+(*   \VV/  **************************************************************)
+(*    //   *      This file is distributed under the terms of the       *)
+(*         *       GNU Lesser General Public License Version 2.1        *)
+(************************************************************************)
+
+(* Morphism instances for relations.
+ 
+   Author: Matthieu Sozeau
+   Institution: LRI, CNRS UMR 8623 - UniversitÃcopyright Paris Sud
+   91405 Orsay, France *)
+
+(** Morphisms for relations *)
+
+Instance relation_conjunction_morphism : Morphism (relation_equivalence (A:=A) ==>
+  relation_equivalence ==> relation_equivalence) relation_conjunction.
+  Proof. firstorder. Qed.
+
+Instance relation_disjunction_morphism : Morphism (relation_equivalence (A:=A) ==>
+  relation_equivalence ==> relation_equivalence) relation_disjunction.
+  Proof. firstorder. Qed.
+
+(* Predicate equivalence is exactly the same as the pointwise lifting of [iff]. *)
+
+Require Import List.
+
+Lemma predicate_equivalence_pointwise (l : list Type) :
+  Morphism (@predicate_equivalence l ==> lift_pointwise l iff) id.
+Proof. do 2 red. unfold predicate_equivalence. auto. Qed.
+
+Lemma predicate_implication_pointwise (l : list Type) :
+  Morphism (@predicate_implication l ==> lift_pointwise l impl) id.
+Proof. do 2 red. unfold predicate_implication. auto. Qed.
+
+(** The instanciation at relation allows to rewrite applications of relations [R x y] to [R' x y] *)
+(*    when [R] and [R'] are in [relation_equivalence]. *)
+
+Instance relation_equivalence_pointwise :
+  Morphism (relation_equivalence ==> pointwise_relation (A:=A) (pointwise_relation (A:=A) iff)) id.
+Proof. apply (predicate_equivalence_pointwise (l:=(cons A (cons A nil)))). Qed.
+
+Instance subrelation_pointwise :
+  Morphism (subrelation ==> pointwise_relation (A:=A) (pointwise_relation (A:=A) impl)) id.
+Proof. apply (predicate_implication_pointwise (l:=(cons A (cons A nil)))). Qed.
